Refactor into more reusable lemmas

src/high/resources/auth_map_map.v
@@ -1,4 +1,6 @@
 From iris.algebra Require Import auth gmap.
+From iris.base_logic.lib Require Import own ghost_map.
+From iris.proofmode Require Import proofmode.
 
 From self.lang Require Import lang.
 From self Require Import extra.
@@ -9,14 +11,10 @@ Definition auth_map_mapR (A : ofe) :=
 Definition fmap_fmap_to_agree_ol (m : gmap loc (gmap time positive)) : gmapUR loc _ :=
   (λ n : gmap _ _, to_agree <$> n) <$> m.
 
-(* Set Printing All. *)
-(* Print fmap_fmap_to_agree_ol. *)
-(* positiveO *)
-
 Section fmap_fmap_to_agree.
-  Context {A : Type}.
+  Context {A : ofe}.
 
-  Definition fmap_fmap_to_agree (m : gmap loc (gmap time A)) : gmapUR loc (gmapUR time (agreeR (leibnizO A))) :=
+  Definition fmap_fmap_to_agree (m : gmap loc (gmap time A)) : gmap loc (gmap time (agreeR A)) :=
     (λ n : gmap _ _, (to_agree) <$> n) <$> m.
 
   Lemma fmap_fmap_to_agree_valid m : ✓ fmap_fmap_to_agree m.
@@ -27,10 +25,10 @@ Section fmap_fmap_to_agree.
     destruct (m !! i); last done.
     simpl.
     apply Some_valid.
-    apply (valid_to_agree_fmap (B := leibnizO A)).
+    apply valid_to_agree_fmap.
   Qed.
 
-  Lemma fmap_fmap_to_agree_incl (* `{!LeibnizEquiv A} *) m m' :
+  Lemma fmap_fmap_to_agree_incl `{!LeibnizEquiv A} m m' :
     dom (gset _) m ⊆ dom _ m' →
     (∀ ℓ mi mi', m !! ℓ = Some mi → m' !! ℓ = Some mi' → mi ⊆ mi') →
     (fmap_fmap_to_agree m) ≼ (fmap_fmap_to_agree m').
@@ -48,8 +46,66 @@ Section fmap_fmap_to_agree.
          set_solver. }
     simpl.
     apply Some_included_total.
-    apply (to_agree_fmap (A := leibnizO A)).
+    apply to_agree_fmap.
     eapply subIn; done.
   Qed.
 
+  Lemma fmap_fmap_to_agree_singleton ℓ h :
+    fmap_fmap_to_agree {[ℓ := h]} = {[ℓ := to_agree <$> h]}.
+  Proof. by rewrite /fmap_fmap_to_agree map_fmap_singleton. Qed.
+
 End fmap_fmap_to_agree.
+
+Section auth_map_map.
+  Context {A : ofe}.
+  Context `{inG Σ (auth_map_mapR A)}.
+
+  Implicit Types (m : gmap loc (gmap time A)).
+
+  Definition auth_map_map_auth γ m :=
+    own γ (● (fmap_fmap_to_agree m)).
+
+  Definition auth_map_map_frag γ m :=
+    own γ (◯ (fmap_fmap_to_agree m)).
+
+  Definition auth_map_map_frag_singleton γ ℓ t a :=
+    auth_map_map_frag γ {[ ℓ := {[ t := a ]} ]}.
+
+  (* NOTE: The requirement on leibniz equiv may not be strictly necessary, but
+  it is convenient right now. *)
+  Lemma auth_map_map_insert `{!LeibnizEquiv A} γ m ℓ t h a :
+    m !! ℓ = Some h →
+    h !! t = None →
+    auth_map_map_auth γ m ==∗
+    auth_map_map_auth γ (<[ℓ:=<[t:=a]> h]> m) ∗
+      auth_map_map_frag_singleton γ ℓ t a.
+  Proof.
+    iIntros (mLook hLook) "N".
+    iMod (own_update with "N ") as "H".
+    2: {
+      iMod (own_update with "H") as "[$ $]".
+      { apply: auth_update_dfrac_alloc.
+        rewrite /fmap_fmap_to_agree.
+        rewrite -> fmap_insert.
+        rewrite map_fmap_singleton.
+        apply singleton_included_insert.
+        apply to_agree_fmap.
+        apply map_singleton_subseteq_l.
+        apply lookup_insert. }
+      done. }
+    { apply auth_auth_grow.
+      { apply fmap_fmap_to_agree_valid. }
+      apply fmap_fmap_to_agree_incl.
+      * set_solver.
+      * intros ℓ' mi mi' look1 look2.
+        destruct (decide (ℓ = ℓ')).
+        + simplify_eq.
+          rewrite lookup_insert in look2.
+          simplify_eq.
+          by apply insert_subseteq.
+        + rewrite lookup_insert_ne in look2; last done.
+          simplify_eq.
+          reflexivity. }
+  Qed.
+
+End auth_map_map.
